##### FRQ 1
a)
$$
ma=-mg-bv
$$
$$
m \frac{dv}{dt} = -mg-bv
$$
$$
\frac{dv}{dt} = \frac{-mg-bv}{m}
$$
$$
\frac{dv}{-mg-bv} = \frac{dt}{m}
$$
$$
\frac{dv}{-b\left( v+\frac{mg}{b} \right)} = \frac{dt}{m}
$$
$$
\frac{dv}{v+\frac{mg}{b}} = -\frac{b}{m}dt
$$
$$
\int_{v_{0}}^v \frac{dv}{v+\frac{mg}{b}} = \int_{0}^t -\frac{b}{m}dt
$$
$$
\ln\left( v+\frac{mg}{b} \right) \biggr|_{v_{0}}^v = -\frac{b}{m}t
$$
$$
\ln\left( v+\frac{mg}{b} \right) - \ln\left( v_{0}+\frac{mg}{b} \right) = -\frac{bt}{m}
$$
$$
\ln\left( v+\frac{mg}{b} \right) = \ln\left( v_{0}+\frac{mg}{b} \right)-\frac{bt}{m}
$$
$$
v+\frac{mg}{b} = e^{\ln\left( v_{0}+\frac{mg}{b} \right)-\frac{bt}{m}} = \left( v_{0}+\frac{mg}{b} \right)e^{-\frac{bt}{m}}
$$
$$
v=\left( v_{0}+\frac{mg}{b} \right)e^{-\frac{bt}{m}}-\frac{mg}{b}
$$

$$
-mg-bv
$$
b) Starts below $-g$ and increases concave down to $-g$ at $th$ then continues to 0 concave down
c)

$$
v=0=\left( v_{0}+\frac{mg}{b} \right)e^{-\frac{bt}{m}}-\frac{mg}{b}
$$
$$
\frac{mg}{b} = \left( v_{0}+\frac{mg}{b} \right)e^{-\frac{bt}{m}}
$$
$$
\frac{mg}{b\left( v_{0}+\frac{mg}{b} \right)} = e^{-\frac{bt}{m}}
$$
$$
\ln\left( \frac{mg}{b\left( v_{0}+\frac{mg}{b} \right)} \right) = -\frac{bt}{m}
$$
$$
\ln\left( \frac{b\left( v_{0}+\frac{mg}{b} \right)}{mg} \right) = \frac{bt}{m}
$$
$$
t=\frac{m}{b}\ln\left( \frac{b\left( v_{0}+\frac{mg}{b} \right)}{mg} \right) 
$$
##### FRQ 2
a) Both blocks will have $F_{g}$ arrow pointing straight down though block b should have a smaller arrow. Block A has $F_{n}$ arrow which points perpendicular from the plane towards the top right. Block A also has $F_{T}$ arrow pointing down the plane, parallel to the plane. Block B has $F_{T}$ arrow which points directly upwards

b)
$$
\sum F_{block_{a}} = 4Ma = 4Mg\sin \theta+F_{T}
$$
$$
\sum F_{block_{b}} = Ma = Mg-F_{T}
$$
$$
\sum F = 5Ma = Mg+4Mg\sin \theta
$$
$$
a = \frac{g+4g\sin \theta}{5}
$$
c) Block a: since $\sin \theta$ increases concave down as it approaches 90°, The shape would be the same but the Net Force at each angle would be less because the $F_{g}$ from block b is in the same direction down the incline so it increases the net force. If block b were to be removed, the net force of block a would be just its gravity compenet parallel to the plane.

d) The graph for block a would start at a force of zero as there would be no force acting horizontally and the upward normal force balances the gravitational force. The graph would increase with angle and still be 4Mg at 90° because Block A would be in free fall.

##### FRQ 4
a) Yes, the box would come to a complete stop in a finite amount of time. The opposing force, $F_{a}$ will reduce over time since it is indirectly proportional to time. This means that it will decrease over time and also at a rapid pace. The force of kinetic friction, however, is not dependent on time and will stay constant. Eventually, the force of kinetic friciton will overcome the force applied, causing the box to accelerate to the right, leading it to come to a complete stop.

b) 
$$
\sum F = Ma = F_{0}e^{-Bt}-\mu_{k}Mg
$$
$$
M \frac{dv}{dt} = F_{0}e^{-Bt}-\mu_{k}Mg
$$
$$
\frac{dv}{dt} = \frac{F_{0}e^{-Bt}-\mu_{k}Mg}{M}
$$
$$
dv = \frac{F_{0}e^{-Bt}-\mu_{k}Mg}{M} dt
$$
$$
\int_{v_{0}}^v dv = \int_{0}^t \frac{F_{0}e^{-Bt}-\mu_{k}Mg}{M} dt
$$
$$
v-v_{0} = \frac{1}{M} \left(-\frac{F_{0}e^{-Bt}}{B} -\mu_{k}Mgt \right) \Biggr|_{0}^t
$$
$$
v-v_{0} = \frac{1}{M}\left(-\frac{F_{0}e^{-Bt}}{B} -\mu_{k}Mgt + \frac{F_{0}}{B} \right) 
$$
$$
v=\frac{1}{M}\left(-\frac{F_{0}e^{-Bt}}{B} -\mu_{k}Mgt + \frac{F_{0}}{B} \right) +v_{0}
$$
c) The equation for the velocity derived is consistent with the reasoning in part a that as time passes, the box will eventually come to a stop. In the equation, as t becomes greater, the expression $-\mu_{k}Mgt$ will continue to become greater in magnitude, eventually becoming greater than $\frac{F_{0}}{B}$ resulting in a negative change in velocity until the block stops.


$$
\sum F = ma = F\cos \theta-mg\sin(\theta)-F_{fr}
$$
$$
\mu = \frac{F_{fr}}{F_{n}}
$$
$$
F_{n} = F\sin \theta+
$$
$$
\sum F = ma = T-\mu_{k}mg
$$
$$
T=ma+\mu_{k}mg
$$
$$
F_{c} = m \frac{v^2}{r} = F_{T}-mg
$$

$$
\sum F = ma = F\cos \theta - \mu(mg+F\sin \theta)
$$
$$
F\cos \theta-\mu F\sin \theta=ma+\mu mg
$$

$$
F=ma=m \left( \frac{v_{f}-v_{0}}{\Delta t} \right)
$$

$$
F_{fk} = ma = \mu mg
$$
$$
\frac{v^2}{r} = \frac{Gm_{sun}}{r^2}
$$
$$
M \to \frac{M}{8}
$$
$$
mg\sin \theta
$$
$$
\sum F=ma=F_{a}-\mu_{k} 20
$$
$$
\sum F=ma=mg\sin \theta-\mu mg\cos \theta
$$
$$
\sum F=(M+m)a=Mg-mg
$$
$$
a=\frac{M-m}{M+m}g
$$
$$
ma=mg\sin \theta
$$
$$
v_{f}^2=2a(\Delta x)
$$
$$
\frac{v^2}{r}
$$
$$
F_{app} = mg\sin \theta
$$
$$
F_{c}=F_{T}-mg
$$
$$
a_{c}=\frac{v^2}{r}=\frac{F_{T}}{m}-g
$$
$$
v=\sqrt{ r\left( \frac{F_{T}}{m}-g \right) }
$$

$$
\frac{4\pi^2r^2}{T^2}=\frac{GM}{r^2}
$$
